Fix proofs by leaving sorrys

Semantic/ModalCapybara/TypeSystem/Core.lean
@@ -182,6 +182,7 @@ inductive HasType : CaptureSet s -> Ctx s -> Exp s -> Ty .exi s -> Prop where
   -----------------------------
   HasType {} Γ (.cabs cs cb e) (.typ (.cpoly cb cs T))
 | wrap :
+  Ψ.IsClosed ->
   HasType
     (cs.rename Rename.succ) (Γ.push_lock Ψ)
     (e.rename Rename.succ) (E.rename Rename.succ) ->
